src/contracts_coq/vote.v
@@ -25,7 +25,6 @@ Require Import ZArith.
 Import error.
 Require List.
 Require tez.
-Require int64.
 Require map.
 
 Definition parameter_ty : type := string.
@@ -79,6 +78,11 @@ Definition vote_spec
               end
   | None => True end).
 
+Lemma l1 a b : tez.compare a b = Z.compare (tez.to_Z a) (tez.to_Z b).
+Proof.
+  reflexivity.
+Defined.
+
 Theorem vote_correct
       (storage : data storage_ty)
       (param : data parameter_ty)
@@ -94,104 +98,78 @@ Proof.
   rewrite return_precond.
   rewrite eval_precond_correct.
   do 15 (more_fuel; simplify_instruction).
-
-  destruct (BinInt.Z.gtb
-      (comparison_to_int
-         (tez.compare
-            (exist (fun t : int64.int64 => int64.sign t = false)
-               (int64.of_Z 5000000) eq_refl) (amount env))) 0) eqn:gtamount.
-
-  - (* Not enough tez sent to contract *)
-    split; intros;
-      unfold tez.compare, comparison_to_int in gtamount; simpl in gtamount.
-    + inversion H.
-    + unfold vote_spec in H. destruct H as [gtamountcontra _].
-      destruct (int64.compare (int64.of_Z 5000000) (tez.to_int64 (amount env))) eqn:amount;
-        try inversion gtamount.
-      exfalso. clear gtamount. 
-      unfold tez.to_Z in gtamountcontra.
-      unfold tez.to_int64 in *. destruct (E.amount env) as [t _].
-      apply Z.compare_ge_iff in gtamountcontra.
-      apply gtamountcontra. clear gtamountcontra.
-      unfold int64.compare, int64.of_Z, int64.to_Z at 1 in amount.
-      rewrite Zdigits.Z_to_two_compl_to_Z in amount. assumption.
-      simpl. omega. reflexivity.
+  rewrite if_false_not.
+  apply and_both_0.
+  - change (tez.compare (5000000 ~Mutez) (amount env)) with
+        (5000000 ?= (tez.to_Z (amount env)))%Z.
+    rewrite Z.compare_antisym.
+    unfold ">="%Z.
+    destruct (tez.to_Z (amount env) ?= 5000000)%Z; simpl; intuition discriminate.
   - (* Enough tez sent to contract *)
     destruct (map.get str Z string_compare param storage) eqn:mapget.
     + (* Key is in the map *)
       more_fuel; simplify_instruction.
       split; intros.
       * (* ->  *)
-        unfold vote_spec; repeat split.
-        { clear H. clear mapget.
-          unfold tez.compare, tez.to_int64 in gtamount.
-          unfold tez.to_Z. unfold tez.to_int64.
-          destruct (amount env) as [t _].
-          destruct (int64.compare (int64.of_Z 5000000) t) eqn:cp;
-            unfold int64.compare in cp;
-            simpl in gtamount; try inversion gtamount;
-          unfold int64.compare, int64.of_Z, int64.to_Z at 1 in cp;
-          rewrite Zdigits.Z_to_two_compl_to_Z in cp by (try (simpl; omega); try reflexivity);
-          rewrite Z.ge_le_iff; unfold Z.le; rewrite cp; discriminate. }
-        unfold get, semantics.get. simpl.
-        apply map.map_getmem with z. assumption.
-        { inversion H. intro Hstor.
-          unfold get, semantics.get. simpl.
-          apply map.map_updatemem. assumption. }
-        { inversion H. intro Hnstor.
-          unfold get, semantics.get in Hnstor. simpl in Hnstor.
-          unfold get, semantics.get. simpl.
-          destruct (string_compare s param) eqn:strcomp.
-          rewrite string_compare_Eq_correct in strcomp; subst.
-          apply map.map_getmem with z. assumption.
-          eapply map.map_updatemem_rev with (k':= param).
-          rewrite <- (compare_diff string). left. eassumption. eassumption.
-          eapply map.map_updatemem_rev with (k':= param).
-          rewrite <- (compare_diff string). right. eassumption. eassumption. }
-        { inversion H. reflexivity. }
-        { unfold get, semantics.get. simpl. rewrite mapget.
-          inversion H.
-          rewrite map.map_updateeq.
-          destruct z; try destruct p; reflexivity. }
-        { intros s Hneq. unfold get, semantics.get. simpl.
-          inversion H.
-          destruct (map.get str Z string_compare s storage) eqn:mapget2.
-          rewrite map.map_updateneq.
-          rewrite mapget2. reflexivity. intro contra. subst; contradiction.
-          exact I. }
+        simpl in *.
+        repeat split; inversion H.
+        -- apply map.map_getmem with z; assumption.
+        -- intro Hstor.
+           apply map.map_updatemem.
+           assumption.
+        -- intro Hnstor.
+           destruct (string_compare s param) eqn:strcomp.
+           rewrite string_compare_Eq_correct in strcomp; subst.
+           apply map.map_getmem with z. assumption.
+           eapply map.map_updatemem_rev with (k':= param).
+           rewrite <- (compare_diff string). left. eassumption. eassumption.
+           eapply map.map_updatemem_rev with (k':= param).
+           rewrite <- (compare_diff string). right. eassumption. eassumption.
+        -- reflexivity.
+        -- rewrite mapget.
+           rewrite map.map_updateeq.
+           destruct z; try destruct p; reflexivity.
+        -- intros s Hneq.
+           destruct (map.get str Z string_compare s storage) eqn:mapget2.
+           rewrite map.map_updateneq.
+           rewrite mapget2. reflexivity. intro contra. subst; contradiction.
+           constructor.
       * (* <- *)
         repeat simplify_instruction.
-        destruct H as [H1 [H2 [H3 [H4 [H5 H6]]]]].
-        f_equal. f_equal. symmetry. simpl. assumption.
-        symmetry. rewrite map.map_updateSome_spec. split. 
-        clear H6. unfold get, semantics.get in H5; simpl in H5.
-        destruct (map.get str Z string_compare param storage);
-          destruct (map.get str Z string_compare param new_storage); subst;
-            try inversion H5.
-        inversion mapget; subst. rewrite BinInt.Z.add_comm. reflexivity.
-        clear H5.
-        intros s Hdiff. specialize (H6 s).
-        assert (s <> param) as Hdiff2 by (intro contra; rewrite contra in Hdiff; contradiction);
-        apply H6 in Hdiff2.
-        unfold get, semantics.get in Hdiff2. simpl in Hdiff2.
-        destruct (map.get str Z string_compare s storage) eqn:get1;
-          destruct (map.get str Z string_compare s new_storage) eqn:get2; subst;
-            try reflexivity.
-        inversion Hdiff2.
-        exfalso. clear H6.
-        apply map.map_getmem in get2.
-        unfold mem, semantics.mem in H3; simpl in H3.
-        rewrite <- H3 in get2. apply map.map_memget in get2. destruct get2 as [v get2].
-        rewrite get2 in get1. discriminate get1.
-    + (* Key is not in the map *)
-      more_fuel; simplify_instruction.
-      split; intros.
+        destruct H as [H1 [H2 [H3 [H4 H5]]]].
+        repeat f_equal.
+        -- symmetry. assumption.
+        -- symmetry.
+           rewrite map.map_updateSome_spec.
+           split.
+           ++ unfold get, semantics.get in H5; simpl in H5.
+              simpl in *.
+              destruct (map.get str Z string_compare param storage); destruct (map.get str Z string_compare param new_storage); subst;
+                try inversion H4.
+              inversion mapget; subst. rewrite BinInt.Z.add_comm. reflexivity.
+           ++ simpl in *.
+              clear H4.
+              intros s Hdiff. specialize (H5 s).
+              assert (s <> param) as Hdiff2 by (intro contra; rewrite contra in Hdiff; contradiction);
+                apply H5 in Hdiff2.
+              unfold get, semantics.get in Hdiff2. simpl in Hdiff2.
+              destruct (map.get str Z string_compare s storage) eqn:get1;
+                destruct (map.get str Z string_compare s new_storage) eqn:get2; subst;
+                  try reflexivity.
+              inversion Hdiff2.
+              exfalso. clear H5.
+              apply map.map_getmem in get2.
+              rewrite <- H2 in get2. apply map.map_memget in get2. destruct get2 as [v get2].
+              rewrite get2 in get1. discriminate get1.
+  + (* Key is not in the map *)
+    more_fuel; simplify_instruction.
+               split; intros.
       * (* -> *)
         inversion H.
       * (* <- *)
-        destruct H as [H1 [H2 [H3 [H4 [H5 H6]]]]].
-        apply map.map_memget in H2. destruct H2 as [v H2].
-        simpl in H2. rewrite H2 in mapget. discriminate mapget.
+        destruct H as [H1 [H2 [H3 [H4 H5]]]].
+        apply map.map_memget in H1. destruct H1 as [v H1].
+        simpl in H1. rewrite H1 in mapget. discriminate mapget.
 Qed.
 
 End vote.
