src/michocoq/error_pp.v
@@ -1,0 +1,26 @@
+Require Import location error String micheline_pp ZArith.
+
+Open Scope string.
+
+Definition location_pp (l : location) : string :=
+  "line " ++ string_of_Z (Z.of_nat l.(line)) ++ " column " ++ string_of_Z (Z.of_nat l.(column)).
+
+
+Definition exception_pp (e : exception) : string :=
+  match e with
+  | Out_of_fuel => "Out of execution fuel"
+  | Overflow => "Overflow"
+  | Assertion_Failure _ _ => "Assertion failure"
+  | Lexing l => "Lexing error at " ++ location_pp l
+  | Parsing => "Parsing error"
+  | Parsing_Out_of_Fuel => "Out of parsing fuel"
+  | Expansion b e => "Expansion error between " ++ location_pp b ++ " and " ++ location_pp e
+  | Expansion_prim b e s => "Unknown primitive " ++ s ++ " between " ++ location_pp b ++ " and " ++ location_pp e
+  | Typing _ _ => "Typing error"
+  end.
+
+Definition m_pp {A} (m : M A) : string :=
+  match m with
+  | Return _ _ => "OK"
+  | Failed _ e => exception_pp e
+  end.
