src/michocoq/extraction/extraction.v
@@ -18,11 +18,86 @@
 (* LIABILITY, WHETHER IN AN ACTION OF CONTRACT, TORT OR OTHERWISE, ARISING *)
 (* FROM, OUT OF OR IN CONNECTION WITH THE SOFTWARE OR THE USE OR OTHER *)
 (* DEALINGS IN THE SOFTWARE. *)
-
-
 Require Extraction.
-Require Import Michocoq.semantics.
-Recursive Extraction Library semantics.
+Require ExtrOcamlBasic.
+Require ExtrOcamlString.
 
-Require Import Michocoq.typer.
-Recursive Extraction Library typer.
+Extract Constant Ascii.ascii_of_pos => "(fun x -> Char.chr (Zarith.to_int x))".
+
+
+(* Require Import Michocoq.semantics. *)
+(* Recursive Extraction Library semantics. *)
+Require Import Michocoq.comparable Michocoq.int64bv Michocoq.typer Michocoq.micheline_lexer Michocoq.micheline_parser
+Michocoq.micheline2michelson Michocoq.main.
+(* Recursive Extraction Library micheline_lexer. *)
+(* Recursive Extraction Library micheline_parser. *)
+
+Extract Inlined Constant ascii_compare => "(fun c1 c2 -> if (c1 < c2) then cl else if (c1 > c2) then Gt else Eq)".
+
+Require Import ZArith NArith.
+
+(* Mapping Z to the OCaml library Zarith. *)
+Extract Inductive positive =>
+"Zarith.t"
+  [ "(fun x -> Zarith.add Zarith.one (Zarith.mul (Zarith.add Zarith.one Zarith.one) x))" "(fun x -> Zarith.mul (Zarith.add Zarith.one Zarith.one) x)" "Zarith.one" ]
+  "(fun b1 b2 b3 x -> Zarith.(if x = one then b3 () else let (q, r) = ediv_rem x (of_int 2) in if r = zero then b2 q else b1 q))".
+
+Extract Inductive Z =>
+"Zarith.t"
+  [ "Zarith.zero" "" "Zarith.neg" ]
+  "(fun b1 b2 b3 x -> Zarith.(if x > zero then b2 x else if x < zero then b3 x else b1 ()))".
+
+Extract Inductive N => "Zarith.t"
+ [ "Zarith.zero" "" ] "(fun b1 b2 x -> Zarith.(if x > zero then b2 x else b1 ()))".
+
+Extract Constant Pos.add => "Zarith.add".
+Extract Constant Pos.succ => "Zarith.succ".
+Extract Constant Pos.pred => "fun n -> Zarith.(max one (pred n))".
+Extract Constant Pos.sub => "fun n m -> Zarith.(max one (sub n m))".
+Extract Constant Pos.mul => "Zarith.mul".
+Extract Constant Pos.min => "Zarith.min".
+Extract Constant Pos.max => "Zarith.max".
+Extract Constant Pos.compare =>
+ "fun x y -> Zarith.(if x < y then Lt else if x > y then Gt else Eq)".
+Extract Constant Pos.compare_cont =>
+ "fun c x y -> Zarith.(if x < y then Lt else if x > y then Gt else c)".
+
+Extract Constant N.add => "Zarith.add".
+Extract Constant N.succ => "Zarith.succ".
+Extract Constant N.pred => "fun n -> Zarith.(max zero (pred n))".
+Extract Constant N.sub => "fun n m -> Zarith.(max zero (sub n m))".
+Extract Constant N.mul => "Zarith.mul".
+Extract Constant N.min => "Zarith.min".
+Extract Constant N.max => "Zarith.max".
+Extract Constant N.div =>
+ "fun a b -> Zarith.(if b = zero then zero else Zarith.div a b)".
+Extract Constant N.modulo =>
+ "fun a b -> Zarith.(if b = zero then zero else Zarith.rem a b)".
+Extract Constant N.compare =>
+ "fun x y -> Zarith.(if x < y then Lt else if x > y then Gt else Eq)".
+
+Extract Constant Z.add => "Zarith.add".
+Extract Constant Z.succ => "Zarith.succ".
+Extract Constant Z.pred => "Zarith.pred".
+Extract Constant Z.sub => "Zarith.sub".
+Extract Constant Z.mul => "Zarith.mul".
+Extract Constant Z.opp => "Zarith.neg".
+Extract Constant Z.abs => "Zarith.abs".
+Extract Constant Z.min => "Zarith.min".
+Extract Constant Z.max => "Zarith.max".
+Extract Constant Z.compare => "fun x y -> Zarith.(if x < y then Lt else if x > y then Gt else Eq)".
+
+Extract Constant Z.of_N => "fun p -> p".
+Extract Constant Z.abs_N => "Zarith.abs".
+
+Extract Constant Zdigits.Zmod2 => "fun x -> Zarith.ediv x (Zarith.add Zarith.one Zarith.one)".
+
+Extract Inlined Constant int64 => "int64".
+Extract Inlined Constant sign => "(fun x -> Int64.compare x 0L < 0)".
+Extract Inlined Constant to_Z => "Zarith.of_int64".
+Extract Inlined Constant of_Z => "Zarith.to_int64".
+
+Recursive Extraction Library main.
+
+(* Require Import Michocoq.main. *)
+(* Recursive Extraction Library main. *)
