src/michocoq/main.v
@@ -1,9 +1,18 @@
 Require Import String ZArith.
 Require micheline_lexer micheline_parser.
-Require untyped_syntax micheline2michelson typer.
+Require micheline2michelson typer.
 Require syntax.
 Require Import syntax_type.
+Require dummy_contract_context.
+Require error_pp.
 
+Module syntax := syntax.Syntax(dummy_contract_context).
+Module typer := typer.Typer(dummy_contract_context).
+Import typer syntax.
+
+Section Main.
+  Variable input : String.string.
+  Variable fuel : Datatypes.nat.
 
 Definition wrap_parser_result {A} r : error.M A :=
   match r with
@@ -15,188 +24,66 @@ Definition wrap_parser_result {A} r : error.M A :=
     error.Return _ m
   end.
 
-Definition parse_micheline fuel (s : micheline_parser.MenhirLibParser.Inter.buffer)
-  : error.M micheline_syntax.loc_micheline :=
-  wrap_parser_result (micheline_parser.file fuel s).
+Definition lexed_M := micheline_lexer.lex_micheline_to_parser input.
 
-Definition lex_and_parse_micheline fuel input :
-  error.M (micheline_syntax.loc_micheline) :=
+Definition parsed_M :=
   error.bind
-    (parse_micheline fuel)
-    (micheline_lexer.lex_micheline_to_parser input).
+    (fun x => wrap_parser_result (micheline_parser.seq_file fuel x))
+    lexed_M.
 
-Definition lex_and_parse_and_expand_type fuel input
-  : error.M type :=
-  error.bind
-    (fun m => micheline2michelson.micheline2michelson_type m)
-    (lex_and_parse_micheline fuel input).
-
-Definition get_file_object_from_string fuel input :=
+Definition michelson_M :=
   error.bind
     micheline2michelson.micheline2michelson_file
-    (error.bind
-       (fun x => wrap_parser_result (micheline_parser.seq_file fuel x))
-       (micheline_lexer.lex_micheline_to_parser input)).
+    parsed_M.
 
-Definition get_parameter_type_from_string fuel input :=
+Definition self_type_M :=
   error.bind
     (fun a => error.Return _ a.(micheline2michelson.parameter))
-    (get_file_object_from_string fuel input).
+    michelson_M.
 
-Definition get_storage_type_from_string fuel input :=
+Definition storage_type_M :=
   error.bind
     (fun a => error.Return _ a.(micheline2michelson.storage))
-    (get_file_object_from_string fuel input).
+    michelson_M.
 
-Module Type PARSEDSELFTYPE.
-  Parameter input : String.string.
-  Parameter fuel : Datatypes.nat.
-  Parameter success_param : error.Is_true (error.success (get_parameter_type_from_string fuel input)).
-  Parameter success_storage : error.Is_true (error.success (get_storage_type_from_string fuel input)).
-End PARSEDSELFTYPE.
+Definition contract_file_M : error.M syntax.contract_file :=
+  error.bind
+    (fun self_type =>
+       error.bind
+         (fun storage_type =>
+            error.bind
+              (fun '(existT _ tff code) =>
+                 error.Return
+                   _
+                   {| contract_file_parameter := self_type;
+                      contract_file_storage := storage_type;
+                      contract_tff := tff;
+                      contract_file_code := code; |})
+              (error.bind
+                 (fun i =>
+                    typer.type_check_instruction typer.type_instruction i _ _)
+                 (error.bind
+                    (fun a => error.Return _ a.(micheline2michelson.code))
+                    michelson_M)))
+         storage_type_M)
+    self_type_M.
 
-Module Type PARSEDFILE <: semantics.SelfType.
-  Parameter file_object : error.M micheline2michelson.untyped_michelson_file.
-  Parameter self_type : type.
-  Parameter storage_type : type.
-End PARSEDFILE.
+Definition is_lexed := error_pp.m_pp lexed_M.
 
-Module ParsedFile (ParsedSelfType : PARSEDSELFTYPE) <: PARSEDFILE.
-  Definition file_object := get_file_object_from_string ParsedSelfType.fuel ParsedSelfType.input.
-  Definition self_type :=
-    error.extract (error.bind (fun a => error.Return _ a.(micheline2michelson.parameter)) file_object)
-                  ParsedSelfType.success_param.
-  Definition storage_type :=
-    error.extract (error.bind (fun a => error.Return _ a.(micheline2michelson.storage)) file_object)
-                  ParsedSelfType.success_storage.
-End ParsedFile.
+Definition is_parsed := error_pp.m_pp parsed_M.
 
-Module Main(ST : PARSEDFILE).
+Definition is_michelson := error_pp.m_pp michelson_M.
 
-  (* Dummy context: getting the type of a contract always fails. *)
-  Module ContractContext.
-    Definition get_contract_type (_ : syntax.contract_constant) :
-      Datatypes.option type := None.
-  End ContractContext.
+Definition type_check := error_pp.m_pp contract_file_M.
 
-  Module syntax := syntax.Syntax(ContractContext).
-  Module typer := typer.Typer(ContractContext).
-  Import typer. Import syntax.
+Definition fixed_fuel : Datatypes.nat := 500.
 
-  Definition full_contract := syntax.full_contract.
+Definition lf := micheline_pp.lf.
 
-  Definition code_M : error.M untyped_syntax.instruction :=
-    error.bind
-      (fun a => error.Return _ a.(micheline2michelson.code))
-      ST.file_object.
-
-  Definition lex_and_parse_and_expand_and_type_full_contract
-    : error.M (syntax.full_contract ST.self_type ST.storage_type) :=
-         error.bind
-           (fun i =>
-              typer.type_check_instruction_no_tail_fail typer.type_instruction i _ _)
-           code_M.
-
-  Definition type_check : Datatypes.bool := error.success lex_and_parse_and_expand_and_type_full_contract.
+Definition print_info :=
+  ("Lexing: " ++ is_lexed ++ lf ++
+   "Parsing: " ++ is_parsed ++ lf ++
+   "Expansion: " ++ is_michelson ++ lf ++
+   "Type checking: " ++ type_check ++ lf)%string.
 
 End Main.
-
-Module MultisigParsedSelfType <: PARSEDSELFTYPE.
-  Definition input : String.string :=
-    "
-parameter (pair
-             (pair :payload
-                (nat %counter) # counter, used to prevent replay attacks
-                (or :action    # payload to sign, represents the requested action
-                   (pair :transfer    # transfer tokens
-                      (mutez %amount) # amount to transfer
-                      (contract %dest unit)) # destination to transfer to
-                   (or
-                      (option %delegate key_hash) # change the delegate to this address
-                      (pair %change_keys          # change the keys controlling the multisig
-                         (nat %threshold)         # new threshold
-                         (list %keys key)))))     # new list of keys
-             (list %sigs (option signature)));    # signatures
-
-storage (pair (nat %stored_counter) (pair (nat %threshold) (list %keys key))) ;
-
-code
-  {
-    UNPAIR ; SWAP ; DUP ; DIP { SWAP } ;
-    DIP
-      {
-        UNPAIR ;
-        # pair the payload with the current contract address, to ensure signatures
-        # can't be replayed accross different contracts if a key is reused.
-        DUP ; SELF ; ADDRESS ; PAIR ;
-        PACK ; # form the binary payload that we expect to be signed
-        DIP { UNPAIR @counter ; DIP { SWAP } } ; SWAP
-      } ;
-
-    # Check that the counters match
-    UNPAIR @stored_counter; DIP { SWAP };
-    ASSERT_CMPEQ ;
-
-    # Compute the number of valid signatures
-    DIP { SWAP } ; UNPAIR @threshold @keys;
-    DIP
-      {
-        # Running count of valid signatures
-        PUSH @valid nat 0; SWAP ;
-        ITER
-          {
-            DIP { SWAP } ; SWAP ;
-            IF_CONS
-              {
-                IF_SOME
-                  { SWAP ;
-                    DIP
-                      {
-                        SWAP ; DIIP { DIP { DUP } ; SWAP } ;
-                        # Checks signatures, fails if invalid
-                        CHECK_SIGNATURE ; ASSERT ;
-                        PUSH nat 1 ; ADD @valid } }
-                  { SWAP ; DROP }
-              }
-              {
-                # There were fewer signatures in the list
-                # than keys. Not all signatures must be present, but
-                # they should be marked as absent using the option type.
-                FAIL
-              } ;
-            SWAP
-          }
-      } ;
-    # Assert that the threshold is less than or equal to the
-    # number of valid signatures.
-    ASSERT_CMPLE ;
-    DROP ; DROP ;
-
-    # Increment counter and place in storage
-    DIP { UNPAIR ; PUSH nat 1 ; ADD @new_counter ; PAIR} ;
-
-    # We have now handled the signature verification part,
-    # produce the operation requested by the signers.
-    NIL operation ; SWAP ;
-    IF_LEFT
-      { # Transfer tokens
-        UNPAIR ; UNIT ; TRANSFER_TOKENS ; CONS }
-      { IF_LEFT {
-                  # Change delegate
-                  SET_DELEGATE ; CONS }
-                {
-                  # Change set of signatures
-                  DIP { SWAP ; CAR } ; SWAP ; PAIR ; SWAP }} ;
-    PAIR }".
-
-  Definition fuel := 600.
-
-  Definition success_param := I.
-  Definition success_storage := I.
-End MultisigParsedSelfType.
-
-Module MultisigParsedFile := ParsedFile MultisigParsedSelfType.
-Module MultisigMain := Main MultisigParsedFile.
-
-Lemma multisig_type_check : Bool.Is_true MultisigMain.type_check.
-Proof. exact I. Qed.
