src/michocoq/dummy_contract_context.v
@@ -1,0 +1,4 @@
+Require syntax.
+Require syntax_type.
+Definition get_contract_type (_ : syntax.contract_constant) :
+  Datatypes.option syntax_type.type := None.
